soundness: extract F* model for Scalar

ristretto255/proofs/fstar/extraction/Ristretto255.Scalar.fst
@@ -7,77 +7,791 @@ let _ =
   (* This module has implicit dependencies, here we make them explicit. *)
   (* The implicit dependencies arise from typeclasses instances. *)
   let open Rand_core in
+  let open Subtle in
   ()
 
 /// A scalar value for the ristretto255 group.
 /// Scalars are integers mod ℓ, where ℓ is the order of the ristretto255 group.
 type t_Scalar = | Scalar : t_Array u8 (mk_usize 32) -> t_Scalar
 
-let impl_1: Core_models.Clone.t_Clone t_Scalar =
+let impl_2: Core_models.Clone.t_Clone t_Scalar =
   { f_clone = (fun x -> x); f_clone_pre = (fun _ -> True); f_clone_post = (fun _ _ -> True) }
 
 [@@ FStar.Tactics.Typeclasses.tcinstance]
 assume
-val impl_2': Core_models.Fmt.t_Debug t_Scalar
-
-unfold
-let impl_2 = impl_2'
-
-[@@ FStar.Tactics.Typeclasses.tcinstance]
-assume
-val impl_3': Core_models.Marker.t_StructuralPartialEq t_Scalar
+val impl_3': Core_models.Fmt.t_Debug t_Scalar
 
 unfold
 let impl_3 = impl_3'
 
 [@@ FStar.Tactics.Typeclasses.tcinstance]
 assume
-val impl_4': Core_models.Cmp.t_PartialEq t_Scalar t_Scalar
+val impl_4': Core_models.Marker.t_StructuralPartialEq t_Scalar
 
 unfold
 let impl_4 = impl_4'
 
 [@@ FStar.Tactics.Typeclasses.tcinstance]
 assume
-val impl_5': Core_models.Cmp.t_Eq t_Scalar
+val impl_5': Core_models.Cmp.t_PartialEq t_Scalar t_Scalar
 
 unfold
 let impl_5 = impl_5'
 
-/// Generate a random scalar using the provided RNG.
+[@@ FStar.Tactics.Typeclasses.tcinstance]
 assume
-val impl_Scalar__random':
-    #v_R: Type0 ->
-    {| i0: Rand_core.t_RngCore v_R |} ->
-    {| i1: Rand_core.t_CryptoRng v_R |} ->
-    e_rng: v_R
-  -> (v_R & t_Scalar)
+val impl_6': Core_models.Cmp.t_Eq t_Scalar
 
 unfold
-let impl_Scalar__random
-      (#v_R: Type0)
-      (#[FStar.Tactics.Typeclasses.tcresolve ()] i0: Rand_core.t_RngCore v_R)
-      (#[FStar.Tactics.Typeclasses.tcresolve ()] i1: Rand_core.t_CryptoRng v_R)
-     = impl_Scalar__random' #v_R #i0 #i1
+let impl_6 = impl_6'
 
-/// Attempt to construct a scalar from a canonical byte representation.
-/// Returns `None` if the bytes do not represent a canonical scalar
-/// (i.e. the value is >= ℓ).
+/// Serialize this scalar to a 32-byte little-endian array.
+let impl_Scalar__to_bytes (self: t_Scalar) : t_Array u8 (mk_usize 32) = self._0
+
+/// `Scalar52` represents an element of ℤ/ℓℤ as 5 × 52-bit limbs.
+type t_Scalar52 = | Scalar52 : t_Array u64 (mk_usize 5) -> t_Scalar52
+
+let impl_8: Core_models.Clone.t_Clone t_Scalar52 =
+  { f_clone = (fun x -> x); f_clone_pre = (fun _ -> True); f_clone_post = (fun _ _ -> True) }
+
+[@@ FStar.Tactics.Typeclasses.tcinstance]
 assume
-val impl_Scalar__from_bytes_checked': e_bytes: t_Array u8 (mk_usize 32)
-  -> Core_models.Option.t_Option t_Scalar
+val impl_7': Core_models.Marker.t_Copy t_Scalar52
 
 unfold
-let impl_Scalar__from_bytes_checked = impl_Scalar__from_bytes_checked'
+let impl_7 = impl_7'
+
+/// u64 × u64 → u128 multiply helper.
+let m (x y: u64) : u128 = (cast (x <: u64) <: u128) *! (cast (y <: u64) <: u128)
+
+let impl_Scalar52__ZERO: t_Scalar52 =
+  Scalar52
+  (let list = [mk_u64 0; mk_u64 0; mk_u64 0; mk_u64 0; mk_u64 0] in
+    FStar.Pervasives.assert_norm (Prims.eq2 (List.Tot.length list) 5);
+    Rust_primitives.Hax.array_of_list 5 list)
+  <:
+  t_Scalar52
+
+let impl_Scalar52__from_bytes (bytes: t_Array u8 (mk_usize 32)) : t_Scalar52 =
+  let words:t_Array u64 (mk_usize 4) = Rust_primitives.Hax.repeat (mk_u64 0) (mk_usize 4) in
+  let words:t_Array u64 (mk_usize 4) =
+    Rust_primitives.Hax.Folds.fold_range (mk_usize 0)
+      (mk_usize 4)
+      (fun words temp_1_ ->
+          let words:t_Array u64 (mk_usize 4) = words in
+          let _:usize = temp_1_ in
+          true)
+      words
+      (fun words i ->
+          let words:t_Array u64 (mk_usize 4) = words in
+          let i:usize = i in
+          Rust_primitives.Hax.Folds.fold_range (mk_usize 0)
+            (mk_usize 8)
+            (fun words temp_1_ ->
+                let words:t_Array u64 (mk_usize 4) = words in
+                let _:usize = temp_1_ in
+                true)
+            words
+            (fun words j ->
+                let words:t_Array u64 (mk_usize 4) = words in
+                let j:usize = j in
+                Rust_primitives.Hax.Monomorphized_update_at.update_at_usize words
+                  i
+                  ((words.[ i ] <: u64) |.
+                    ((cast (bytes.[ (i *! mk_usize 8 <: usize) +! j <: usize ] <: u8) <: u64) <<!
+                      (j *! mk_usize 8 <: usize)
+                      <:
+                      u64)
+                    <:
+                    u64)
+                <:
+                t_Array u64 (mk_usize 4))
+          <:
+          t_Array u64 (mk_usize 4))
+  in
+  let mask:u64 = (mk_u64 1 <<! mk_i32 52 <: u64) -! mk_u64 1 in
+  let top_mask:u64 = (mk_u64 1 <<! mk_i32 48 <: u64) -! mk_u64 1 in
+  Scalar52
+  (let list =
+      [
+        (words.[ mk_usize 0 ] <: u64) &. mask;
+        (((words.[ mk_usize 0 ] <: u64) >>! mk_i32 52 <: u64) |.
+          ((words.[ mk_usize 1 ] <: u64) <<! mk_i32 12 <: u64)
+          <:
+          u64) &.
+        mask;
+        (((words.[ mk_usize 1 ] <: u64) >>! mk_i32 40 <: u64) |.
+          ((words.[ mk_usize 2 ] <: u64) <<! mk_i32 24 <: u64)
+          <:
+          u64) &.
+        mask;
+        (((words.[ mk_usize 2 ] <: u64) >>! mk_i32 28 <: u64) |.
+          ((words.[ mk_usize 3 ] <: u64) <<! mk_i32 36 <: u64)
+          <:
+          u64) &.
+        mask;
+        ((words.[ mk_usize 3 ] <: u64) >>! mk_i32 16 <: u64) &. top_mask
+      ]
+    in
+    FStar.Pervasives.assert_norm (Prims.eq2 (List.Tot.length list) 5);
+    Rust_primitives.Hax.array_of_list 5 list)
+  <:
+  t_Scalar52
+
+let impl_Scalar52__to_bytes (self: t_Scalar52) : t_Array u8 (mk_usize 32) =
+  let s:t_Array u8 (mk_usize 32) = Rust_primitives.Hax.repeat (mk_u8 0) (mk_usize 32) in
+  let s:t_Array u8 (mk_usize 32) =
+    Rust_primitives.Hax.Monomorphized_update_at.update_at_usize s
+      (mk_usize 0)
+      (cast ((self._0.[ mk_usize 0 ] <: u64) >>! mk_i32 0 <: u64) <: u8)
+  in
+  let s:t_Array u8 (mk_usize 32) =
+    Rust_primitives.Hax.Monomorphized_update_at.update_at_usize s
+      (mk_usize 1)
+      (cast ((self._0.[ mk_usize 0 ] <: u64) >>! mk_i32 8 <: u64) <: u8)
+  in
+  let s:t_Array u8 (mk_usize 32) =
+    Rust_primitives.Hax.Monomorphized_update_at.update_at_usize s
+      (mk_usize 2)
+      (cast ((self._0.[ mk_usize 0 ] <: u64) >>! mk_i32 16 <: u64) <: u8)
+  in
+  let s:t_Array u8 (mk_usize 32) =
+    Rust_primitives.Hax.Monomorphized_update_at.update_at_usize s
+      (mk_usize 3)
+      (cast ((self._0.[ mk_usize 0 ] <: u64) >>! mk_i32 24 <: u64) <: u8)
+  in
+  let s:t_Array u8 (mk_usize 32) =
+    Rust_primitives.Hax.Monomorphized_update_at.update_at_usize s
+      (mk_usize 4)
+      (cast ((self._0.[ mk_usize 0 ] <: u64) >>! mk_i32 32 <: u64) <: u8)
+  in
+  let s:t_Array u8 (mk_usize 32) =
+    Rust_primitives.Hax.Monomorphized_update_at.update_at_usize s
+      (mk_usize 5)
+      (cast ((self._0.[ mk_usize 0 ] <: u64) >>! mk_i32 40 <: u64) <: u8)
+  in
+  let s:t_Array u8 (mk_usize 32) =
+    Rust_primitives.Hax.Monomorphized_update_at.update_at_usize s
+      (mk_usize 6)
+      (cast (((self._0.[ mk_usize 0 ] <: u64) >>! mk_i32 48 <: u64) |.
+            ((self._0.[ mk_usize 1 ] <: u64) <<! mk_i32 4 <: u64)
+            <:
+            u64)
+        <:
+        u8)
+  in
+  let s:t_Array u8 (mk_usize 32) =
+    Rust_primitives.Hax.Monomorphized_update_at.update_at_usize s
+      (mk_usize 7)
+      (cast ((self._0.[ mk_usize 1 ] <: u64) >>! mk_i32 4 <: u64) <: u8)
+  in
+  let s:t_Array u8 (mk_usize 32) =
+    Rust_primitives.Hax.Monomorphized_update_at.update_at_usize s
+      (mk_usize 8)
+      (cast ((self._0.[ mk_usize 1 ] <: u64) >>! mk_i32 12 <: u64) <: u8)
+  in
+  let s:t_Array u8 (mk_usize 32) =
+    Rust_primitives.Hax.Monomorphized_update_at.update_at_usize s
+      (mk_usize 9)
+      (cast ((self._0.[ mk_usize 1 ] <: u64) >>! mk_i32 20 <: u64) <: u8)
+  in
+  let s:t_Array u8 (mk_usize 32) =
+    Rust_primitives.Hax.Monomorphized_update_at.update_at_usize s
+      (mk_usize 10)
+      (cast ((self._0.[ mk_usize 1 ] <: u64) >>! mk_i32 28 <: u64) <: u8)
+  in
+  let s:t_Array u8 (mk_usize 32) =
+    Rust_primitives.Hax.Monomorphized_update_at.update_at_usize s
+      (mk_usize 11)
+      (cast ((self._0.[ mk_usize 1 ] <: u64) >>! mk_i32 36 <: u64) <: u8)
+  in
+  let s:t_Array u8 (mk_usize 32) =
+    Rust_primitives.Hax.Monomorphized_update_at.update_at_usize s
+      (mk_usize 12)
+      (cast ((self._0.[ mk_usize 1 ] <: u64) >>! mk_i32 44 <: u64) <: u8)
+  in
+  let s:t_Array u8 (mk_usize 32) =
+    Rust_primitives.Hax.Monomorphized_update_at.update_at_usize s
+      (mk_usize 13)
+      (cast ((self._0.[ mk_usize 2 ] <: u64) >>! mk_i32 0 <: u64) <: u8)
+  in
+  let s:t_Array u8 (mk_usize 32) =
+    Rust_primitives.Hax.Monomorphized_update_at.update_at_usize s
+      (mk_usize 14)
+      (cast ((self._0.[ mk_usize 2 ] <: u64) >>! mk_i32 8 <: u64) <: u8)
+  in
+  let s:t_Array u8 (mk_usize 32) =
+    Rust_primitives.Hax.Monomorphized_update_at.update_at_usize s
+      (mk_usize 15)
+      (cast ((self._0.[ mk_usize 2 ] <: u64) >>! mk_i32 16 <: u64) <: u8)
+  in
+  let s:t_Array u8 (mk_usize 32) =
+    Rust_primitives.Hax.Monomorphized_update_at.update_at_usize s
+      (mk_usize 16)
+      (cast ((self._0.[ mk_usize 2 ] <: u64) >>! mk_i32 24 <: u64) <: u8)
+  in
+  let s:t_Array u8 (mk_usize 32) =
+    Rust_primitives.Hax.Monomorphized_update_at.update_at_usize s
+      (mk_usize 17)
+      (cast ((self._0.[ mk_usize 2 ] <: u64) >>! mk_i32 32 <: u64) <: u8)
+  in
+  let s:t_Array u8 (mk_usize 32) =
+    Rust_primitives.Hax.Monomorphized_update_at.update_at_usize s
+      (mk_usize 18)
+      (cast ((self._0.[ mk_usize 2 ] <: u64) >>! mk_i32 40 <: u64) <: u8)
+  in
+  let s:t_Array u8 (mk_usize 32) =
+    Rust_primitives.Hax.Monomorphized_update_at.update_at_usize s
+      (mk_usize 19)
+      (cast (((self._0.[ mk_usize 2 ] <: u64) >>! mk_i32 48 <: u64) |.
+            ((self._0.[ mk_usize 3 ] <: u64) <<! mk_i32 4 <: u64)
+            <:
+            u64)
+        <:
+        u8)
+  in
+  let s:t_Array u8 (mk_usize 32) =
+    Rust_primitives.Hax.Monomorphized_update_at.update_at_usize s
+      (mk_usize 20)
+      (cast ((self._0.[ mk_usize 3 ] <: u64) >>! mk_i32 4 <: u64) <: u8)
+  in
+  let s:t_Array u8 (mk_usize 32) =
+    Rust_primitives.Hax.Monomorphized_update_at.update_at_usize s
+      (mk_usize 21)
+      (cast ((self._0.[ mk_usize 3 ] <: u64) >>! mk_i32 12 <: u64) <: u8)
+  in
+  let s:t_Array u8 (mk_usize 32) =
+    Rust_primitives.Hax.Monomorphized_update_at.update_at_usize s
+      (mk_usize 22)
+      (cast ((self._0.[ mk_usize 3 ] <: u64) >>! mk_i32 20 <: u64) <: u8)
+  in
+  let s:t_Array u8 (mk_usize 32) =
+    Rust_primitives.Hax.Monomorphized_update_at.update_at_usize s
+      (mk_usize 23)
+      (cast ((self._0.[ mk_usize 3 ] <: u64) >>! mk_i32 28 <: u64) <: u8)
+  in
+  let s:t_Array u8 (mk_usize 32) =
+    Rust_primitives.Hax.Monomorphized_update_at.update_at_usize s
+      (mk_usize 24)
+      (cast ((self._0.[ mk_usize 3 ] <: u64) >>! mk_i32 36 <: u64) <: u8)
+  in
+  let s:t_Array u8 (mk_usize 32) =
+    Rust_primitives.Hax.Monomorphized_update_at.update_at_usize s
+      (mk_usize 25)
+      (cast ((self._0.[ mk_usize 3 ] <: u64) >>! mk_i32 44 <: u64) <: u8)
+  in
+  let s:t_Array u8 (mk_usize 32) =
+    Rust_primitives.Hax.Monomorphized_update_at.update_at_usize s
+      (mk_usize 26)
+      (cast ((self._0.[ mk_usize 4 ] <: u64) >>! mk_i32 0 <: u64) <: u8)
+  in
+  let s:t_Array u8 (mk_usize 32) =
+    Rust_primitives.Hax.Monomorphized_update_at.update_at_usize s
+      (mk_usize 27)
+      (cast ((self._0.[ mk_usize 4 ] <: u64) >>! mk_i32 8 <: u64) <: u8)
+  in
+  let s:t_Array u8 (mk_usize 32) =
+    Rust_primitives.Hax.Monomorphized_update_at.update_at_usize s
+      (mk_usize 28)
+      (cast ((self._0.[ mk_usize 4 ] <: u64) >>! mk_i32 16 <: u64) <: u8)
+  in
+  let s:t_Array u8 (mk_usize 32) =
+    Rust_primitives.Hax.Monomorphized_update_at.update_at_usize s
+      (mk_usize 29)
+      (cast ((self._0.[ mk_usize 4 ] <: u64) >>! mk_i32 24 <: u64) <: u8)
+  in
+  let s:t_Array u8 (mk_usize 32) =
+    Rust_primitives.Hax.Monomorphized_update_at.update_at_usize s
+      (mk_usize 30)
+      (cast ((self._0.[ mk_usize 4 ] <: u64) >>! mk_i32 32 <: u64) <: u8)
+  in
+  let s:t_Array u8 (mk_usize 32) =
+    Rust_primitives.Hax.Monomorphized_update_at.update_at_usize s
+      (mk_usize 31)
+      (cast ((self._0.[ mk_usize 4 ] <: u64) >>! mk_i32 40 <: u64) <: u8)
+  in
+  s
+
+let impl_Scalar52__mul_internal (a b: t_Scalar52) : t_Array u128 (mk_usize 9) =
+  let a:t_Array u64 (mk_usize 5) = a._0 in
+  let b:t_Array u64 (mk_usize 5) = b._0 in
+  let list =
+    [
+      m (a.[ mk_usize 0 ] <: u64) (b.[ mk_usize 0 ] <: u64);
+      (m (a.[ mk_usize 0 ] <: u64) (b.[ mk_usize 1 ] <: u64) <: u128) +!
+      (m (a.[ mk_usize 1 ] <: u64) (b.[ mk_usize 0 ] <: u64) <: u128);
+      ((m (a.[ mk_usize 0 ] <: u64) (b.[ mk_usize 2 ] <: u64) <: u128) +!
+        (m (a.[ mk_usize 1 ] <: u64) (b.[ mk_usize 1 ] <: u64) <: u128)
+        <:
+        u128) +!
+      (m (a.[ mk_usize 2 ] <: u64) (b.[ mk_usize 0 ] <: u64) <: u128);
+      (((m (a.[ mk_usize 0 ] <: u64) (b.[ mk_usize 3 ] <: u64) <: u128) +!
+          (m (a.[ mk_usize 1 ] <: u64) (b.[ mk_usize 2 ] <: u64) <: u128)
+          <:
+          u128) +!
+        (m (a.[ mk_usize 2 ] <: u64) (b.[ mk_usize 1 ] <: u64) <: u128)
+        <:
+        u128) +!
+      (m (a.[ mk_usize 3 ] <: u64) (b.[ mk_usize 0 ] <: u64) <: u128);
+      ((((m (a.[ mk_usize 0 ] <: u64) (b.[ mk_usize 4 ] <: u64) <: u128) +!
+            (m (a.[ mk_usize 1 ] <: u64) (b.[ mk_usize 3 ] <: u64) <: u128)
+            <:
+            u128) +!
+          (m (a.[ mk_usize 2 ] <: u64) (b.[ mk_usize 2 ] <: u64) <: u128)
+          <:
+          u128) +!
+        (m (a.[ mk_usize 3 ] <: u64) (b.[ mk_usize 1 ] <: u64) <: u128)
+        <:
+        u128) +!
+      (m (a.[ mk_usize 4 ] <: u64) (b.[ mk_usize 0 ] <: u64) <: u128);
+      (((m (a.[ mk_usize 1 ] <: u64) (b.[ mk_usize 4 ] <: u64) <: u128) +!
+          (m (a.[ mk_usize 2 ] <: u64) (b.[ mk_usize 3 ] <: u64) <: u128)
+          <:
+          u128) +!
+        (m (a.[ mk_usize 3 ] <: u64) (b.[ mk_usize 2 ] <: u64) <: u128)
+        <:
+        u128) +!
+      (m (a.[ mk_usize 4 ] <: u64) (b.[ mk_usize 1 ] <: u64) <: u128);
+      ((m (a.[ mk_usize 2 ] <: u64) (b.[ mk_usize 4 ] <: u64) <: u128) +!
+        (m (a.[ mk_usize 3 ] <: u64) (b.[ mk_usize 3 ] <: u64) <: u128)
+        <:
+        u128) +!
+      (m (a.[ mk_usize 4 ] <: u64) (b.[ mk_usize 2 ] <: u64) <: u128);
+      (m (a.[ mk_usize 3 ] <: u64) (b.[ mk_usize 4 ] <: u64) <: u128) +!
+      (m (a.[ mk_usize 4 ] <: u64) (b.[ mk_usize 3 ] <: u64) <: u128);
+      m (a.[ mk_usize 4 ] <: u64) (b.[ mk_usize 4 ] <: u64)
+    ]
+  in
+  FStar.Pervasives.assert_norm (Prims.eq2 (List.Tot.length list) 9);
+  Rust_primitives.Hax.array_of_list 9 list
+
+let impl_Scalar52__montgomery_reduce__part2 (sum: u128) : (u128 & u64) =
+  let w:u64 = (cast (sum <: u128) <: u64) &. ((mk_u64 1 <<! mk_i32 52 <: u64) -! mk_u64 1 <: u64) in
+  sum >>! mk_i32 52, w <: (u128 & u64)
+
+/// `L` is the group order ℓ = 2^252 + 27742317777372353535851937790883648493.
+let v_L: t_Scalar52 =
+  Scalar52
+  (let list =
+      [
+        mk_u64 671914833335277;
+        mk_u64 3916664325105025;
+        mk_u64 1367801;
+        mk_u64 0;
+        mk_u64 17592186044416
+      ]
+    in
+    FStar.Pervasives.assert_norm (Prims.eq2 (List.Tot.length list) 5);
+    Rust_primitives.Hax.array_of_list 5 list)
+  <:
+  t_Scalar52
+
+let impl_Scalar52__sub (a b: t_Scalar52) : t_Scalar52 =
+  let difference:t_Scalar52 = impl_Scalar52__ZERO in
+  let mask:u64 = (mk_u64 1 <<! mk_i32 52 <: u64) -! mk_u64 1 in
+  let (borrow: u64):u64 = mk_u64 0 in
+  let (borrow: u64), (difference: t_Scalar52) =
+    Rust_primitives.Hax.Folds.fold_range (mk_usize 0)
+      (mk_usize 5)
+      (fun temp_0_ temp_1_ ->
+          let (borrow: u64), (difference: t_Scalar52) = temp_0_ in
+          let _:usize = temp_1_ in
+          true)
+      (borrow, difference <: (u64 & t_Scalar52))
+      (fun temp_0_ i ->
+          let (borrow: u64), (difference: t_Scalar52) = temp_0_ in
+          let i:usize = i in
+          let borrow:u64 =
+            Core_models.Num.impl_u64__wrapping_sub (a._0.[ i ] <: u64)
+              ((b._0.[ i ] <: u64) +! (borrow >>! mk_i32 63 <: u64) <: u64)
+          in
+          let difference:t_Scalar52 =
+            {
+              difference with
+              _0
+              =
+              Rust_primitives.Hax.Monomorphized_update_at.update_at_usize difference._0
+                i
+                (borrow &. mask <: u64)
+            }
+            <:
+            t_Scalar52
+          in
+          borrow, difference <: (u64 & t_Scalar52))
+  in
+  let underflow:Subtle.t_Choice =
+    Core_models.Convert.f_from #Subtle.t_Choice
+      #u8
+      #FStar.Tactics.Typeclasses.solve
+      (cast (borrow >>! mk_i32 63 <: u64) <: u8)
+  in
+  let (carry: u64):u64 = mk_u64 0 in
+  let (carry: u64), (difference: t_Scalar52) =
+    Rust_primitives.Hax.Folds.fold_range (mk_usize 0)
+      (mk_usize 5)
+      (fun temp_0_ temp_1_ ->
+          let (carry: u64), (difference: t_Scalar52) = temp_0_ in
+          let _:usize = temp_1_ in
+          true)
+      (carry, difference <: (u64 & t_Scalar52))
+      (fun temp_0_ i ->
+          let (carry: u64), (difference: t_Scalar52) = temp_0_ in
+          let i:usize = i in
+          let addend:u64 =
+            Subtle.f_conditional_select #u64
+              #FStar.Tactics.Typeclasses.solve
+              (mk_u64 0)
+              (v_L._0.[ i ] <: u64)
+              underflow
+          in
+          let carry:u64 =
+            ((carry >>! mk_i32 52 <: u64) +! (difference._0.[ i ] <: u64) <: u64) +! addend
+          in
+          let difference:t_Scalar52 =
+            {
+              difference with
+              _0
+              =
+              Rust_primitives.Hax.Monomorphized_update_at.update_at_usize difference._0
+                i
+                (carry &. mask <: u64)
+            }
+            <:
+            t_Scalar52
+          in
+          carry, difference <: (u64 & t_Scalar52))
+  in
+  difference
+
+let impl_Scalar52__add (a b: t_Scalar52) : t_Scalar52 =
+  let sum:t_Scalar52 = impl_Scalar52__ZERO in
+  let mask:u64 = (mk_u64 1 <<! mk_i32 52 <: u64) -! mk_u64 1 in
+  let (carry: u64):u64 = mk_u64 0 in
+  let (carry: u64), (sum: t_Scalar52) =
+    Rust_primitives.Hax.Folds.fold_range (mk_usize 0)
+      (mk_usize 5)
+      (fun temp_0_ temp_1_ ->
+          let (carry: u64), (sum: t_Scalar52) = temp_0_ in
+          let _:usize = temp_1_ in
+          true)
+      (carry, sum <: (u64 & t_Scalar52))
+      (fun temp_0_ i ->
+          let (carry: u64), (sum: t_Scalar52) = temp_0_ in
+          let i:usize = i in
+          let carry:u64 =
+            ((a._0.[ i ] <: u64) +! (b._0.[ i ] <: u64) <: u64) +! (carry >>! mk_i32 52 <: u64)
+          in
+          let sum:t_Scalar52 =
+            {
+              sum with
+              _0
+              =
+              Rust_primitives.Hax.Monomorphized_update_at.update_at_usize sum._0
+                i
+                (carry &. mask <: u64)
+            }
+            <:
+            t_Scalar52
+          in
+          carry, sum <: (u64 & t_Scalar52))
+  in
+  impl_Scalar52__sub sum v_L
+
+/// `L * LFACTOR ≡ -1  (mod 2^52)`.
+let v_LFACTOR: u64 = mk_u64 1439961107955227
+
+let impl_Scalar52__montgomery_reduce__part1 (sum: u128) : (u128 & u64) =
+  let p:u64 =
+    (Core_models.Num.impl_u64__wrapping_mul (cast (sum <: u128) <: u64) v_LFACTOR <: u64) &.
+    ((mk_u64 1 <<! mk_i32 52 <: u64) -! mk_u64 1 <: u64)
+  in
+  (sum +! (m p (v_L._0.[ mk_usize 0 ] <: u64) <: u128) <: u128) >>! mk_i32 52, p <: (u128 & u64)
+
+let impl_Scalar52__montgomery_reduce (limbs: t_Array u128 (mk_usize 9)) : t_Scalar52 =
+  let l:t_Array u64 (mk_usize 5) = v_L._0 in
+  let (carry: u128), (n0: u64) =
+    impl_Scalar52__montgomery_reduce__part1 (limbs.[ mk_usize 0 ] <: u128)
+  in
+  let (carry: u128), (n1: u64) =
+    impl_Scalar52__montgomery_reduce__part1 ((carry +! (limbs.[ mk_usize 1 ] <: u128) <: u128) +!
+        (m n0 (l.[ mk_usize 1 ] <: u64) <: u128)
+        <:
+        u128)
+  in
+  let (carry: u128), (n2: u64) =
+    impl_Scalar52__montgomery_reduce__part1 (((carry +! (limbs.[ mk_usize 2 ] <: u128) <: u128) +!
+          (m n0 (l.[ mk_usize 2 ] <: u64) <: u128)
+          <:
+          u128) +!
+        (m n1 (l.[ mk_usize 1 ] <: u64) <: u128)
+        <:
+        u128)
+  in
+  let (carry: u128), (n3: u64) =
+    impl_Scalar52__montgomery_reduce__part1 (((carry +! (limbs.[ mk_usize 3 ] <: u128) <: u128) +!
+          (m n1 (l.[ mk_usize 2 ] <: u64) <: u128)
+          <:
+          u128) +!
+        (m n2 (l.[ mk_usize 1 ] <: u64) <: u128)
+        <:
+        u128)
+  in
+  let (carry: u128), (n4: u64) =
+    impl_Scalar52__montgomery_reduce__part1 ((((carry +! (limbs.[ mk_usize 4 ] <: u128) <: u128) +!
+            (m n0 (l.[ mk_usize 4 ] <: u64) <: u128)
+            <:
+            u128) +!
+          (m n2 (l.[ mk_usize 2 ] <: u64) <: u128)
+          <:
+          u128) +!
+        (m n3 (l.[ mk_usize 1 ] <: u64) <: u128)
+        <:
+        u128)
+  in
+  let (carry: u128), (r0: u64) =
+    impl_Scalar52__montgomery_reduce__part2 ((((carry +! (limbs.[ mk_usize 5 ] <: u128) <: u128) +!
+            (m n1 (l.[ mk_usize 4 ] <: u64) <: u128)
+            <:
+            u128) +!
+          (m n3 (l.[ mk_usize 2 ] <: u64) <: u128)
+          <:
+          u128) +!
+        (m n4 (l.[ mk_usize 1 ] <: u64) <: u128)
+        <:
+        u128)
+  in
+  let (carry: u128), (r1: u64) =
+    impl_Scalar52__montgomery_reduce__part2 (((carry +! (limbs.[ mk_usize 6 ] <: u128) <: u128) +!
+          (m n2 (l.[ mk_usize 4 ] <: u64) <: u128)
+          <:
+          u128) +!
+        (m n4 (l.[ mk_usize 2 ] <: u64) <: u128)
+        <:
+        u128)
+  in
+  let (carry: u128), (r2: u64) =
+    impl_Scalar52__montgomery_reduce__part2 ((carry +! (limbs.[ mk_usize 7 ] <: u128) <: u128) +!
+        (m n3 (l.[ mk_usize 4 ] <: u64) <: u128)
+        <:
+        u128)
+  in
+  let (carry: u128), (r3: u64) =
+    impl_Scalar52__montgomery_reduce__part2 ((carry +! (limbs.[ mk_usize 8 ] <: u128) <: u128) +!
+        (m n4 (l.[ mk_usize 4 ] <: u64) <: u128)
+        <:
+        u128)
+  in
+  let r4:u64 = cast (carry <: u128) <: u64 in
+  impl_Scalar52__sub (Scalar52
+      (let list = [r0; r1; r2; r3; r4] in
+        FStar.Pervasives.assert_norm (Prims.eq2 (List.Tot.length list) 5);
+        Rust_primitives.Hax.array_of_list 5 list)
+      <:
+      t_Scalar52)
+    v_L
+
+let impl_Scalar52__montgomery_mul (a b: t_Scalar52) : t_Scalar52 =
+  impl_Scalar52__montgomery_reduce (impl_Scalar52__mul_internal a b <: t_Array u128 (mk_usize 9))
+
+/// `R = 2^260 mod ℓ`, the Montgomery modulus.
+let v_R: t_Scalar52 =
+  Scalar52
+  (let list =
+      [
+        mk_u64 4302102966953709;
+        mk_u64 1049714374468698;
+        mk_u64 4503599278581019;
+        mk_u64 4503599627370495;
+        mk_u64 17592186044415
+      ]
+    in
+    FStar.Pervasives.assert_norm (Prims.eq2 (List.Tot.length list) 5);
+    Rust_primitives.Hax.array_of_list 5 list)
+  <:
+  t_Scalar52
+
+/// Reduce this scalar mod ℓ, returning the canonical representative.
+let impl_Scalar__reduce (self: t_Scalar) : t_Scalar =
+  let x:t_Scalar52 = impl_Scalar52__from_bytes self._0 in
+  let xR:t_Array u128 (mk_usize 9) = impl_Scalar52__mul_internal x v_R in
+  let x_mod_l:t_Scalar52 = impl_Scalar52__montgomery_reduce xR in
+  Scalar (impl_Scalar52__to_bytes x_mod_l) <: t_Scalar
 
 /// Construct a scalar by reducing a 256-bit little-endian integer modulo ℓ.
 /// Unlike [`from_bytes_checked`](Self::from_bytes_checked), this always
 /// succeeds by reducing the input mod the group order.
-assume
-val impl_Scalar__from_bytes_mod_order': e_bytes: t_Array u8 (mk_usize 32) -> t_Scalar
+let impl_Scalar__from_bytes_mod_order (bytes: t_Array u8 (mk_usize 32)) : t_Scalar =
+  impl_Scalar__reduce (Scalar bytes <: t_Scalar)
 
-unfold
-let impl_Scalar__from_bytes_mod_order = impl_Scalar__from_bytes_mod_order'
+let impl_Scalar__is_canonical (self: t_Scalar) : Subtle.t_Choice =
+  Subtle.f_ct_eq #(t_Slice u8)
+    #FStar.Tactics.Typeclasses.solve
+    (self._0 <: t_Slice u8)
+    ((impl_Scalar__reduce self)._0 <: t_Slice u8)
 
-/// Serialize this scalar to a 32-byte little-endian array.
-let impl_Scalar__to_bytes (self: t_Scalar) : t_Array u8 (mk_usize 32) = self._0
+/// Attempt to construct a scalar from a canonical byte representation.
+/// Returns `None` if the bytes do not represent a canonical scalar
+/// (i.e. the value is >= ℓ).
+let impl_Scalar__from_bytes_checked (bytes: t_Array u8 (mk_usize 32))
+    : Core_models.Option.t_Option t_Scalar =
+  let candidate:t_Scalar = Scalar bytes <: t_Scalar in
+  let high_bit_unset:Subtle.t_Choice =
+    Subtle.f_ct_eq #u8
+      #FStar.Tactics.Typeclasses.solve
+      ((bytes.[ mk_usize 31 ] <: u8) >>! mk_i32 7 <: u8)
+      (mk_u8 0)
+  in
+  let is_canonical:Subtle.t_Choice = impl_Scalar__is_canonical candidate in
+  if
+    Core_models.Convert.f_into #Subtle.t_Choice
+      #bool
+      #FStar.Tactics.Typeclasses.solve
+      (Core_models.Ops.Bit.f_bitand #Subtle.t_Choice
+          #Subtle.t_Choice
+          #FStar.Tactics.Typeclasses.solve
+          high_bit_unset
+          is_canonical
+        <:
+        Subtle.t_Choice)
+  then Core_models.Option.Option_Some candidate <: Core_models.Option.t_Option t_Scalar
+  else Core_models.Option.Option_None <: Core_models.Option.t_Option t_Scalar
+
+/// `RR = R^2 mod ℓ`.
+let v_RR: t_Scalar52 =
+  Scalar52
+  (let list =
+      [
+        mk_u64 2764609938444603;
+        mk_u64 3768881411696287;
+        mk_u64 1616719297148420;
+        mk_u64 1087343033131391;
+        mk_u64 10175238647962
+      ]
+    in
+    FStar.Pervasives.assert_norm (Prims.eq2 (List.Tot.length list) 5);
+    Rust_primitives.Hax.array_of_list 5 list)
+  <:
+  t_Scalar52
+
+let impl_Scalar52__from_bytes_wide (bytes: t_Array u8 (mk_usize 64)) : t_Scalar52 =
+  let words:t_Array u64 (mk_usize 8) = Rust_primitives.Hax.repeat (mk_u64 0) (mk_usize 8) in
+  let words:t_Array u64 (mk_usize 8) =
+    Rust_primitives.Hax.Folds.fold_range (mk_usize 0)
+      (mk_usize 8)
+      (fun words temp_1_ ->
+          let words:t_Array u64 (mk_usize 8) = words in
+          let _:usize = temp_1_ in
+          true)
+      words
+      (fun words i ->
+          let words:t_Array u64 (mk_usize 8) = words in
+          let i:usize = i in
+          Rust_primitives.Hax.Folds.fold_range (mk_usize 0)
+            (mk_usize 8)
+            (fun words temp_1_ ->
+                let words:t_Array u64 (mk_usize 8) = words in
+                let _:usize = temp_1_ in
+                true)
+            words
+            (fun words j ->
+                let words:t_Array u64 (mk_usize 8) = words in
+                let j:usize = j in
+                Rust_primitives.Hax.Monomorphized_update_at.update_at_usize words
+                  i
+                  ((words.[ i ] <: u64) |.
+                    ((cast (bytes.[ (i *! mk_usize 8 <: usize) +! j <: usize ] <: u8) <: u64) <<!
+                      (j *! mk_usize 8 <: usize)
+                      <:
+                      u64)
+                    <:
+                    u64)
+                <:
+                t_Array u64 (mk_usize 8))
+          <:
+          t_Array u64 (mk_usize 8))
+  in
+  let mask:u64 = (mk_u64 1 <<! mk_i32 52 <: u64) -! mk_u64 1 in
+  let lo:t_Scalar52 =
+    Scalar52
+    (let list =
+        [
+          (words.[ mk_usize 0 ] <: u64) &. mask;
+          (((words.[ mk_usize 0 ] <: u64) >>! mk_i32 52 <: u64) |.
+            ((words.[ mk_usize 1 ] <: u64) <<! mk_i32 12 <: u64)
+            <:
+            u64) &.
+          mask;
+          (((words.[ mk_usize 1 ] <: u64) >>! mk_i32 40 <: u64) |.
+            ((words.[ mk_usize 2 ] <: u64) <<! mk_i32 24 <: u64)
+            <:
+            u64) &.
+          mask;
+          (((words.[ mk_usize 2 ] <: u64) >>! mk_i32 28 <: u64) |.
+            ((words.[ mk_usize 3 ] <: u64) <<! mk_i32 36 <: u64)
+            <:
+            u64) &.
+          mask;
+          (((words.[ mk_usize 3 ] <: u64) >>! mk_i32 16 <: u64) |.
+            ((words.[ mk_usize 4 ] <: u64) <<! mk_i32 48 <: u64)
+            <:
+            u64) &.
+          mask
+        ]
+      in
+      FStar.Pervasives.assert_norm (Prims.eq2 (List.Tot.length list) 5);
+      Rust_primitives.Hax.array_of_list 5 list)
+    <:
+    t_Scalar52
+  in
+  let hi:t_Scalar52 =
+    Scalar52
+    (let list =
+        [
+          ((words.[ mk_usize 4 ] <: u64) >>! mk_i32 4 <: u64) &. mask;
+          (((words.[ mk_usize 4 ] <: u64) >>! mk_i32 56 <: u64) |.
+            ((words.[ mk_usize 5 ] <: u64) <<! mk_i32 8 <: u64)
+            <:
+            u64) &.
+          mask;
+          (((words.[ mk_usize 5 ] <: u64) >>! mk_i32 44 <: u64) |.
+            ((words.[ mk_usize 6 ] <: u64) <<! mk_i32 20 <: u64)
+            <:
+            u64) &.
+          mask;
+          (((words.[ mk_usize 6 ] <: u64) >>! mk_i32 32 <: u64) |.
+            ((words.[ mk_usize 7 ] <: u64) <<! mk_i32 32 <: u64)
+            <:
+            u64) &.
+          mask;
+          (words.[ mk_usize 7 ] <: u64) >>! mk_i32 20
+        ]
+      in
+      FStar.Pervasives.assert_norm (Prims.eq2 (List.Tot.length list) 5);
+      Rust_primitives.Hax.array_of_list 5 list)
+    <:
+    t_Scalar52
+  in
+  let lo:t_Scalar52 = impl_Scalar52__montgomery_mul lo v_R in
+  let hi:t_Scalar52 = impl_Scalar52__montgomery_mul hi v_RR in
+  impl_Scalar52__add hi lo
+
+/// Construct a scalar by reducing a 512-bit little-endian integer modulo ℓ.
+let impl_Scalar__from_bytes_mod_order_wide (bytes: t_Array u8 (mk_usize 64)) : t_Scalar =
+  Scalar (impl_Scalar52__to_bytes (impl_Scalar52__from_bytes_wide bytes <: t_Scalar52)) <: t_Scalar
+
+/// Generate a random scalar using the provided RNG.
+let impl_Scalar__random
+      (#v_R: Type0)
+      (#[FStar.Tactics.Typeclasses.tcresolve ()] i0: Rand_core.t_RngCore v_R)
+      (#[FStar.Tactics.Typeclasses.tcresolve ()] i1: Rand_core.t_CryptoRng v_R)
+      (rng: v_R)
+    : (v_R & t_Scalar) =
+  let bytes:t_Array u8 (mk_usize 64) = Rust_primitives.Hax.repeat (mk_u8 0) (mk_usize 64) in
+  let (tmp0: v_R), (tmp1: t_Array u8 (mk_usize 64)) =
+    Rand_core.f_fill_bytes #v_R #FStar.Tactics.Typeclasses.solve rng bytes
+  in
+  let rng:v_R = tmp0 in
+  let bytes:t_Array u8 (mk_usize 64) = tmp1 in
+  let _:Prims.unit = () in
+  let hax_temp_output:t_Scalar = impl_Scalar__from_bytes_mod_order_wide bytes in
+  rng, hax_temp_output <: (v_R & t_Scalar)
